lean/CoreModels.lean
@@ -3,3 +3,4 @@ import CoreModels.Core
 import CoreModels.Alloc
 import CoreModels.HaxLib
 import CoreModels.RustPrimitives
+import CoreModels.Spec
