lean/CoreModels/Spec/Core/Array.lean
@@ -1,0 +1,81 @@
+import CoreModels.Core.Funs
+import CoreModels.Spec.Aeneas
+import CoreModels.Spec.Core.Slice
+import CoreModels.Spec.RustPrimitives.Slice
+
+namespace CoreModels
+
+open Aeneas
+open Aeneas.Std hiding namespace core alloc
+open Std.Do WP Result
+set_option mvcgen.warning false
+
+open ScalarElab
+
+uscalar @[spec] theorem «%S».Array.eq_spec {N : Std.Usize} {Q}
+  (a : Array «%S» N) (b : Array «%S» N) (h : (Q.1 (a.val == b.val)).down) :
+  ⦃ ⌜ True ⌝ ⦄
+  core.Array.Insts.CoreCmpPartialEqArray.eq core.«%S».Insts.CoreCmpPartialEq'S a b
+  ⦃ Q ⦄ := by
+  mvcgen -trivial [core.Array.Insts.CoreCmpPartialEqArray.eq,
+    core.Array.Insts.CoreCmpPartialEqArray.eq_loop,
+    core.Array.Insts.CoreCmpPartialEqArray.eq_loop.body, rust_primitives.slice.array_index,
+    core.«%S».Insts.CoreCmpPartialEq'S]
+  case vc1.γ => exact Nat
+  case vc4.termination => exact fun i => N.val - i.val
+  case vc3.rel => exact (· < ·)
+  case vc5.hwf => exact wellFounded_lt
+  case vc2.inv => exact fun i => a.val.take i.val = b.val.take i.val
+  case vc10 =>
+    constructor
+    · simp_all [@List.take_add, @List.take_one, -List.take_append_getElem]
+    · grind
+  · grind
+  · grind
+  · grind
+  · grind
+  · convert h; grind
+  · convert h; grind [List.take_eq_self_iff, List.Vector.length_val]
+
+@[spec]
+theorem Array.index_range_spec
+      {T : Type} {N : Std.Usize} (arr : Std.Array T N)
+      (r : core.ops.range.Range Std.Usize)
+      (h0 : r.start.val < r.end.val) -- TODO: We should be able to allow "≤" here
+      (h1 : r.end.val ≤ N.val) :
+    ⦃ ⌜ True ⌝ ⦄
+    core.Array.Insts.CoreOpsIndexIndex.index
+      (core.Shared0Slice.Insts.CoreOpsIndexIndexRangeUsizeSlice T)
+      arr r
+    ⦃ ⇓ r' => ⌜ r'.val = arr.val.slice r.start.val r.end.val ∧
+                r'.val.length + r.start.val = r.end.val ⌝ ⦄ := by
+  mvcgen [core.Array.Insts.CoreOpsIndexIndex.index, core.array.Array.as_slice,
+      rust_primitives.slice.array_as_slice]
+    <;> grind
+
+/-- This spec for from_fn only works for non-mutating functions. If the function
+mutates, we would need a different spec with a user-provided invariant. -/
+@[spec]
+theorem Array.from_fn_spec
+    {T F : Type} [Inhabited T] (N : Std.Usize)
+    (inst : core.ops.function.FnMut F Std.Usize T) (c : F) (f : Nat → T)
+    (hpure : ∀ k : Nat, k < N.val →
+      ⦃ ⌜ True ⌝ ⦄
+      inst.call_mut c ⟨BitVec.ofNat _ k⟩
+      ⦃ ⇓ r => ⌜ r = (f k, c) ⌝ ⦄) :
+    ⦃ ⌜ True ⌝ ⦄
+    core.array.from_fn N inst c
+    ⦃ ⇓ a => ⌜ ∀ i : Nat, (hi : i < N.val) →
+                a.val[i]'(by grind) = f i ⌝ ⦄ := by
+  unfold CoreModels.core.array.from_fn
+  mvcgen
+  case vc1.hpure k hk =>
+    mvcgen [hpure]
+    grind
+  case vc2.success =>
+    intro hpost i hi
+    apply triple_in_hypothesis _ (hpost i hi)
+    mvcgen [hpure]
+    grind
+
+end CoreModels
