lean/CoreModels/Spec/Core/Iter.lean
@@ -1,0 +1,30 @@
+import CoreModels.Core.Funs
+import CoreModels.Alloc.Funs
+import CoreModels.Spec.Aeneas
+
+namespace CoreModels
+
+open Aeneas
+open Aeneas.Std hiding namespace core alloc
+open Std.Do WP Result
+
+set_option mvcgen.warning false
+
+@[spec]
+theorem core.IteratorRange.next_CoreIterRangeStep_spec {Q} (range : core.ops.range.Range Std.Usize)
+      (h_lt : (h : range.start.val < range.end.val) →
+        ∀ (s : Usize), s.val = range.start.val + 1 →
+        (Q.1 (some range.start, { start := s, «end» := range.end })).down)
+      (h_ge : range.start.val ≥ range.end.val → (Q.1 (none, range)).down) :
+    ⦃ ⌜ True ⌝ ⦄
+    core.IteratorRange.next core.Usize.Insts.CoreIterRangeStep range
+    ⦃ Q ⦄ := by
+  mvcgen [core.IteratorRange.next, core.Usize.Insts.CoreIterRangeStep, uncurry,
+    core.Usize.Insts.CoreCmpPartialOrdUsize, core.mkUPartialOrd,
+    core.Usize.Insts.CoreCloneClone.clone, core.Usize.Insts.CoreIterRangeStep.forward_checked,
+    core.convert.TryFromUTInfallible.Blanket.try_from, core.convert.From.Blanket.from,
+    core.num.Usize.checked_add, core.num.Usize.overflowing_add,
+    rust_primitives.arithmetic.overflowing_add_usize]
+    <;> grind [UScalar.overflowing_add, BitVec.uaddOverflow, UScalar.overflowing_add_eq]
+
+end CoreModels
