lean/CoreModels/Spec/Core/Num.lean
@@ -1,0 +1,25 @@
+import CoreModels.Spec.Aeneas
+
+namespace CoreModels
+
+open Aeneas
+open Aeneas.Std hiding namespace core alloc
+open Std.Do WP Result
+
+set_option mvcgen.warning false
+
+attribute [spec]
+  CoreModels.core.num.U8.from_le_bytes
+  CoreModels.core.num.U16.from_le_bytes
+  CoreModels.core.num.U32.from_le_bytes
+  CoreModels.core.num.U64.from_le_bytes
+  CoreModels.core.num.U128.from_le_bytes
+  CoreModels.core.num.Usize.from_le_bytes
+  CoreModels.core.num.U8.to_le_bytes
+  CoreModels.core.num.U16.to_le_bytes
+  CoreModels.core.num.U32.to_le_bytes
+  CoreModels.core.num.U64.to_le_bytes
+  CoreModels.core.num.U128.to_le_bytes
+  CoreModels.core.num.Usize.to_le_bytes
+
+end CoreModels
