lean/CoreModels/Spec/Core/Slice.lean
@@ -1,0 +1,27 @@
+import CoreModels.Spec.Aeneas
+
+namespace CoreModels
+
+open Aeneas
+open Aeneas.Std hiding namespace core alloc
+open Std.Do WP Result
+
+set_option mvcgen.warning false
+
+attribute [spec]
+  CoreModels.core.slice.Slice.len
+
+@[spec]
+theorem core.Shared0Slice.Insts.CoreOpsIndexIndexRangeUsizeSlice.index_spec
+    {T : Type} (s : Slice T) (r : core.ops.range.Range Std.Usize)
+    (h0 : r.start.val < r.end.val) -- TODO: we should be able to allow "≤"
+    (h1 : r.end.val ≤ s.val.length) :
+    ⦃ ⌜ True ⌝ ⦄
+    core.Shared0Slice.Insts.CoreOpsIndexIndexRangeUsizeSlice.index s r
+    ⦃ ⇓ r' => ⌜ r'.val = s.val.slice r.start.val r.end.val ∧
+                r.start.val + r'.val.length = r.end.val ⌝ ⦄ := by
+  mvcgen [core.Shared0Slice.Insts.CoreOpsIndexIndexRangeUsizeSlice.index,
+    rust_primitives.slice.slice_slice, -Slice.subslice_spec.mvcgen_spec, Slice.subslice]
+    <;> grind
+
+end CoreModels
