lean/CoreModels/Spec/RustPrimitives/Arithmetic.lean
@@ -1,0 +1,25 @@
+import CoreModels.Spec.Aeneas
+
+namespace CoreModels
+
+open Aeneas
+open Aeneas.Std hiding namespace core alloc
+open Std.Do WP Result
+
+set_option mvcgen.warning false
+
+attribute [spec]
+  rust_primitives.arithmetic.from_le_bytes_u8
+  rust_primitives.arithmetic.from_le_bytes_u16
+  rust_primitives.arithmetic.from_le_bytes_u32
+  rust_primitives.arithmetic.from_le_bytes_u64
+  rust_primitives.arithmetic.from_le_bytes_u128
+  rust_primitives.arithmetic.from_le_bytes_usize
+  rust_primitives.arithmetic.to_le_bytes_u8
+  rust_primitives.arithmetic.to_le_bytes_u16
+  rust_primitives.arithmetic.to_le_bytes_u32
+  rust_primitives.arithmetic.to_le_bytes_u64
+  rust_primitives.arithmetic.to_le_bytes_u128
+  rust_primitives.arithmetic.to_le_bytes_usize
+
+end CoreModels
